split CompilerInvariant.v into
- ToplevelLoop.v: All the loop and invariant business
- CompilerInvariant.v: Only the conversion between the two seplog styles:
  + Compiler style (used everywhere until and including ToplevelLoop.v):
    "program p instrs" (includes "verify") and
    "subset (footpr (program p instrs)) (of_list x_addrs)"
  + End2End style (used in CompilerInvariant.v and above):
    "ptsto_bytes p (instrencode instrs)" (needs separate "verify") and
    "forall a, code_start <= a < code_pastend -> a in x_addrs"

and prove all the conversion lemmas needed in the new CompilerInvariant.v

compiler/src/compiler/CompilerInvariant.v
@@ -1,69 +1,22 @@
-Require Export Coq.Lists.List.
-Require Import Coq.ZArith.ZArith.
-Export ListNotations.
-Require Export coqutil.Decidable.
 Require Import coqutil.Tactics.rewr.
-Require        compiler.ExprImp.
-Require Export compiler.FlattenExprDef.
-Require Export compiler.FlattenExpr.
-Require        compiler.FlatImp.
-Require Export riscv.Spec.Decode.
-Require Export riscv.Spec.Machine.
-Require Export riscv.Platform.Run.
-Require Export riscv.Platform.Minimal.
-Require Export riscv.Platform.MetricLogging.
-Require Export riscv.Utility.Monads.
-Require Import riscv.Utility.runsToNonDet.
-Require Export riscv.Platform.MetricRiscvMachine.
-Require Import coqutil.Z.Lia.
-Require Import compiler.NameGen.
-Require Import compiler.StringNameGen.
-Require Export compiler.util.Common.
-Require Export coqutil.Decidable.
-Require Export riscv.Utility.Encode.
-Require Export riscv.Spec.Primitives.
-Require Export riscv.Spec.MetricPrimitives.
-Require Import compiler.GoFlatToRiscv.
-Require Import riscv.Utility.MkMachineWidth.
-Require Export riscv.Proofs.DecodeEncode.
-Require Export riscv.Proofs.EncodeBound.
-Require Export compiler.EmitsValid.
-Require coqutil.Map.SortedList.
-Require Import riscv.Utility.Utility.
-Require Export riscv.Platform.Memory.
-Require Export riscv.Utility.InstructionCoercions.
+Require Import coqutil.Map.Interface coqutil.Map.Properties.
+Require Import coqutil.Word.Interface coqutil.Word.Properties.
+Require Import coqutil.Byte.
+Require Import bedrock2.Array.
+Require Import bedrock2.Map.SeparationLogic.
 Require Import compiler.SeparationLogic.
 Require Import compiler.Simp.
-Require Import compiler.FlattenExprSimulation.
-Require Import compiler.RegRename.
-Require Import compiler.FlatToRiscvSimulation.
-Require Import compiler.Simulation.
-Require Import compiler.RiscvEventLoop.
-Require Import bedrock2.MetricLogging.
-Require Import compiler.FlatToRiscvCommon.
 Require Import compiler.FlatToRiscvFunctions.
-Require Import compiler.DivisibleBy4.
-Require Import compiler.SimplWordExpr.
-Require Import compiler.ForeverSafe.
-Require Export compiler.MemoryLayout.
-Require Import FunctionalExtensionality.
-Require Import coqutil.Tactics.autoforward.
-Require Import compiler.FitsStack.
 Require Import compiler.PipelineWithRename.
 Require Import compiler.ExprImpEventLoopSpec.
+Require Import compiler.ToplevelLoop.
+
 
 Existing Instance riscv.Spec.Machine.DefaultRiscvState.
 
 Open Scope Z_scope.
 
 Local Open Scope ilist_scope.
-
-Local Notation "' x <- a ; f" :=
-  (match (a: option _) with
-   | x => f
-   | _ => None
-   end)
-  (right associativity, at level 70, x pattern).
 
 Local Axiom TODO_sam: False.
 
@@ -72,174 +25,13 @@ Section Pipeline1.
   Context {p: Pipeline.parameters}.
   Context {h: Pipeline.assumptions}.
 
-  Context (ml: MemoryLayout)
-          (mlOk: MemoryLayoutOk ml).
-
-  Let init_sp := word.unsigned ml.(stack_pastend).
-
-(*
-  Lemma get_flatten_functions: forall fname argvars resvars body flattened,
-      map.get srcprog.(funimpls) fname = Some (argvars, resvars, body) ->
-      flatten_functions (2^10) (funimpls srcprog) = Some flattened ->
-      exists body', map.get flattened fname = Some (argvars, resvars, body') /\
-                    flatten_function (2^10) (argvars, resvars, body) = Some (argvars, resvars, body').
-  Proof.
-    unfold flatten_functions.
-    destruct srcprog. destruct sat as [_ _ M0 _ _]. cbn -[flatten_function] in *. clear sat.
-    intros.
-    pose proof (map.map_all_values_fw _ _ _ _ H0 _ _ H) as P.
-    unfold flatten_function in *.
-    simp. eauto.
-  Qed.
-
-  Section Riscv.
-    Context (prog: RenamedProgram).
-
-    (* pc at beginning of loop *)
-    Definition pc_start: word :=
-      word.add ml.(code_start)
-               (word.of_Z (4 * Z.of_nat (List.length (FlatToRiscvDef.init_sp_insts init_sp) +
-                                         List.length (FlatToRiscvDef.init_insts prog)))).
-
-    Definition TODO_frame: mem -> Prop. case TODO_sam. Qed.
-    (* don't unfold and count many times *)
-
-    Definition program_base :=
-      word.add ml.(code_start)
-               (word.of_Z (4 * Z.of_nat (List.length (FlatToRiscvDef.init_sp_insts init_sp) +
-                                         List.length (FlatToRiscvDef.init_insts prog) +
-                                         List.length (FlatToRiscvDef.loop_insts prog) +
-                                         List.length (FlatToRiscvDef.backjump_insts prog)))).
-
-    Definition initCodeGhostConsts: GhostConsts := Build_GhostConsts
-      ml.(stack_pastend)
-      num_stackwords
-      (word.add ml.(code_start)
-                (word.of_Z (4 * Z.of_nat (List.length (FlatToRiscvDef.init_sp_insts init_sp)))))
-      (FlatToRiscvDef.init_insts prog)
-      program_base
-      (FlatToRiscvDef.function_positions prog)
-      prog.(funimpls)
-      prog.(funnames)
-      TODO_frame
-      TODO_frame.
-
-    Definition loopBodyGhostConsts: GhostConsts := Build_GhostConsts
-      ml.(stack_pastend)
-      num_stackwords
-      pc_start
-      (FlatToRiscvDef.loop_insts prog)
-      program_base
-      (FlatToRiscvDef.function_positions prog)
-      prog.(funimpls)
-      prog.(funnames)
-      TODO_frame
-      TODO_frame.
-
-    Lemma main_size_correct:
-      FlatToRiscvDef.main_size prog = (Datatypes.length (FlatToRiscvDef.init_insts prog) +
-                                       Datatypes.length (FlatToRiscvDef.loop_insts prog) + 1)%nat.
-    Proof.
-      unfold FlatToRiscvDef.main_size, FlatToRiscvDef.init_insts, FlatToRiscvDef.loop_insts,
-             FlatToRiscvDef.compile_main.
-      rewrite !app_length. simpl.
-      repeat lazymatch goal with
-             | |- ?L = ?R =>
-               match L with
-               | context[?LL] =>
-                 lazymatch LL with
-                 | Datatypes.length (FlatToRiscvDef.compile_stmt _ ?pos1 ?C) =>
-                   match R with
-                   | context[?RR] =>
-                     lazymatch RR with
-                     | Datatypes.length (FlatToRiscvDef.compile_stmt _ ?pos2 C) =>
-                       progress replace LL with RR by
-                           refine (compile_stmt_length_position_indep _ _ _ _ _)
-                     end
-                   end
-                 end
-               end
-             end.
-      blia.
-    Qed.
-
-  End Riscv.
-*)
-
-  Local Notation source_env := (@Pipeline.string_keyed_map p (list string * list string * Syntax.cmd)).
-
-  (* All riscv machine code, layed out from low to high addresses:
-     - init_sp_insts: initializes stack pointer
-     - init_insts: calls init function
-     - loop_insts: calls loop function
-     - backjump_insts: jumps back to calling loop function
-     - fun_insts: code of compiled functions *)
-  Definition compile_prog(prog: source_env): option (list Instruction * funname_env Z) :=
-    'Some (fun_insts, positions) <- @compile p ml prog;
-    let init_sp_insts := FlatToRiscvDef.compile_lit RegisterNames.sp init_sp in
-    'Some init_pos <- map.get positions "init"%string;
-    'Some loop_pos <- map.get positions "loop"%string;
-    let init_insts := [[Jal RegisterNames.ra (3 * 4 + init_pos)]] in
-    let loop_insts := [[Jal RegisterNames.ra (2 * 4 + loop_pos)]] in
-    let backjump_insts := [[Jal Register0 (-4*Z.of_nat (List.length loop_insts))]] in
-    Some (init_sp_insts ++ init_insts ++ loop_insts ++ backjump_insts ++ fun_insts, positions).
-
-  Context (spec: @ProgramSpec (FlattenExpr.mk_Semantics_params _)).
-
-  Let loop_pos := word.add ml.(code_start)
-         (word.of_Z (4 * (Z.of_nat (List.length (FlatToRiscvDef.compile_lit RegisterNames.sp init_sp))) + 4)).
-
-  Axiom Rdata: mem -> Prop. (* maybe (emp True) will be fine *)
-  Axiom Rexec: mem -> Prop. (* maybe (emp True) will be fine *)
-
-  Definition ll_good(done: bool)(mach: MetricRiscvMachine): Prop :=
-    exists (prog: source_env) (instrs: list Instruction) (positions: funname_env Z) (loop_fun_pos: Z),
-      compile_prog prog = Some (instrs, positions) /\
-      ProgramSatisfiesSpec "init"%string "loop"%string prog spec /\
-      map.get positions "loop"%string = Some loop_fun_pos /\
-      exists mH,
-        isReady spec mach.(getLog) mH /\ goodTrace spec mach.(getLog) /\
-        machine_ok ml.(code_start) loop_fun_pos ml.(stack_start) ml.(stack_pastend) instrs
-                   loop_pos (word.add loop_pos (word.of_Z (if done then 4 else 0))) mH Rdata Rexec mach.
-
-  Definition ll_inv: MetricRiscvMachine -> Prop := runsToGood_Invariant ll_good.
-
-  Add Ring wring : (word.ring_theory (word := Utility.word))
+  Add Ring wring : (word.ring_theory (word := (@Utility.word (@FlatToRiscvDef.FlatToRiscvDef.W (@Pipeline.FlatToRiscvDef_params p)))))
       (preprocess [autorewrite with rew_word_morphism],
-       morphism (word.ring_morph (word := Utility.word)),
+       morphism (word.ring_morph (word := (@Utility.word (@FlatToRiscvDef.FlatToRiscvDef.W (@Pipeline.FlatToRiscvDef_params p))))),
        constants [word_cst]).
 
-  (*
-  Lemma init_code_to_loop_body_transition: forall ren m,
-      compile_inv (related (initCodeGhostConsts ren) (FlatToRiscvDef.main_pos ren) true)
-           (@hl_inv (FlattenExpr.mk_Semantics_params _) _ (funimpls srcprog) (init_code srcprog) spec) m ->
-      compile_inv (related (loopBodyGhostConsts ren) (FlatToRiscvDef.loop_pos ren) false)
-           (@hl_inv (FlattenExpr.mk_Semantics_params _) _ (funimpls srcprog) (loop_body srcprog) spec) m.
-  Proof.
-    intros.
-    unfold hl_inv, compile_inv in *.
-    destruct H as ((((((e & c) & t) & me) & l) & mc) & R). simp.
-    refine (ex_intro _ (_, _, _, _, _, _) _); ssplit; try reflexivity; try eassumption.
-    unfold related in *.
-    case TODO_sam.
-    Unshelve. assumption.
-  Qed.
-  *)
-
-  Lemma compile_prog_to_compile: forall prog instrs positions,
-      compile_prog prog = Some (instrs, positions) ->
-      exists before main,
-        compile ml prog = Some (main, positions) /\
-        instrs = before ++ main.
-  Proof.
-    intros. unfold compile_prog in *. simp. do 2 eexists.
-    split; [reflexivity|].
-    match goal with
-    | |- ?A ++ ?i1 :: ?i2 :: ?i3 :: ?B = ?R => change (A ++ [i1; i2; i3] ++ B = R)
-    end.
-    rewrite app_assoc.
-    reflexivity.
-  Qed.
+  Context (ml: MemoryLayout)
+          (mlOk: MemoryLayoutOk ml).
 
   Lemma instrencode_cons: forall instr instrs,
       instrencode (instr :: instrs) =
@@ -268,27 +60,107 @@ Section Pipeline1.
            constr:(iff1ToEq (array_nil PT SZ start))
          end) in *.
 
-  Definition imem(code_start code_pastend: Semantics.word)(instrs: list Instruction): mem -> Prop :=
+  Definition imem(code_start code_pastend: Semantics.word)(instrs: list Instruction): Semantics.mem -> Prop :=
     (ptsto_bytes code_start (instrencode instrs) *
      mem_available (word.sub code_pastend (word.of_Z (Z.of_nat (List.length (instrencode instrs)))))
                    code_pastend)%sep.
 
-  Local Axiom TODO_andres: False.
-
-  Lemma footpr_imem_range: forall start pastend instrs,
-      subset (footpr (imem start pastend instrs))
-             (fun a => word.unsigned start <= word.unsigned a < word.unsigned pastend).
+  Lemma ptsto_bytes_to_program: forall instrs p_code,
+      word.unsigned p_code mod 4 = 0 ->
+      Forall (fun i => verify i iset) instrs ->
+      iff1 (ptsto_bytes p_code (instrencode instrs))
+           (program p_code instrs).
   Proof.
-    unfold subset, elem_of, footpr, footprint_underapprox, imem. intros.
-    case TODO_andres.
+    induction instrs; intros.
+    - reflexivity.
+    - simp. unfold program in *. rewrite array_cons.
+      specialize (IHinstrs (word.add p_code (word.of_Z 4))).
+      unfold ptsto_instr at 1.
+      unfold truncated_scalar, littleendian, ptsto_bytes, ptsto_bytes.ptsto_bytes.
+      simpl.
+      assert (map.ok Pipeline.mem) as Ok by exact FlatToRiscvCommon.mem_ok. (* PARAMRECORDS *)
+      simpl.
+      rewrite <- IHinstrs; [|DivisibleBy4.solve_divisibleBy4|assumption].
+      wwcancel.
+      cbn [seps].
+      rewrite sep_emp_emp.
+      match goal with
+      | |- iff1 (emp ?P) (emp ?Q) => apply (RunInstruction.iff1_emp P Q)
+      end.
+      split; intros _; try exact I.
+      split; [assumption|reflexivity].
   Qed.
 
+  Lemma ptsto_bytes_range: forall bs start pastend m a v,
+      ptsto_bytes start bs m ->
+      word.unsigned start + Z.of_nat (List.length bs) <= word.unsigned pastend ->
+      map.get m a = Some v ->
+      word.unsigned start <= word.unsigned a < word.unsigned pastend.
+  Proof.
+    assert (map.ok Pipeline.mem) as Ok by exact FlatToRiscvCommon.mem_ok.
+    assert (word.ok FlatImp.word) as Okk by exact word_ok. (* PARAMRECORDS *)
+    induction bs; intros.
+    - simpl in *. unfold emp in *. simp. rewrite map.get_empty in H1. discriminate.
+    - simpl in *.
+      unfold sep in H. simp.
+      specialize IHbs with (1 := Hrr).
+      destr (Z.eqb (word.unsigned a0) (word.unsigned start)). 1: blia.
+      specialize (IHbs pastend a0 v).
+      destruct IHbs as [L R].
+      + rewrite word.unsigned_add. unfold word.wrap.
+        eapply Z.le_trans. 2: eassumption.
+        eapply Z.le_trans
+          with (m := word.unsigned start + word.unsigned (word.of_Z 1) + Z.of_nat (Datatypes.length bs)).
+        * apply Z.add_le_mono_r.
+          apply Z.mod_le.
+          -- repeat match goal with
+                    | |- context [word.unsigned ?w] => unique pose proof (word.unsigned_range w)
+                    end.
+             blia.
+          -- destruct width_cases as [F|F]; simpl in *; rewrite F; reflexivity.
+         * rewrite word.unsigned_of_Z.
+           unfold word.wrap.
+           replace (1 mod 2 ^ FlatImp.width) with 1. 1: blia.
+           simpl.
+           destruct width_cases as [F|F]; simpl in *; rewrite F; reflexivity.
+      + unfold map.split in *. simp.
+        rewrite map.get_putmany_dec in H1.
+        destr (map.get mq a0). 1: congruence.
+        exfalso.
+        unfold ptsto in *. subst mp.
+        rewrite map.get_put_dec in H1.
+        destr (word.eqb start a0).
+        * apply E. congruence.
+        * rewrite map.get_empty in H1. discriminate.
+      + rewrite word.unsigned_add in L. unfold word.wrap in L.
+        split; try assumption.
+        eapply Z.le_trans. 2: eassumption.
+        repeat match goal with
+               | |- context [word.unsigned ?w] => unique pose proof (word.unsigned_range w)
+               end.
+        rewrite Z.mod_small. 1: blia.
+        split; [blia|].
+        eapply Z.le_lt_trans.
+        2: exact (proj2 (word.unsigned_range pastend)).
+        eapply Z.le_trans. 2: eassumption.
+        rewrite word.unsigned_of_Z.
+        unfold word.wrap.
+        replace (1 mod 2 ^ width) with 1. 1: blia.
+        simpl.
+        destruct width_cases as [F|F]; simpl in *; rewrite F; reflexivity.
+  Qed.
+
+  Context (spec: @ProgramSpec (FlattenExpr.mk_Semantics_params _)).
+
   Definition initial_conditions(initial: MetricRiscvMachine): Prop :=
-    exists (srcprog: source_env) (instrs: list Instruction) (positions: funname_env Z),
+    exists (srcprog: Semantics.env) (instrs: list Instruction) (positions: FlatToRiscvCommon.funname_env Z),
       ProgramSatisfiesSpec "init"%string "loop"%string srcprog spec /\
       spec.(datamem_start) = ml.(heap_start) /\
       spec.(datamem_pastend) = ml.(heap_pastend) /\
-      compile_prog srcprog = Some (instrs, positions) /\
+      compile_prog ml srcprog = Some (instrs, positions) /\
+      word.unsigned ml.(code_start) + Z.of_nat (List.length (instrencode instrs)) <=
+        word.unsigned ml.(code_pastend) /\
+      Forall (fun i : Instruction => verify i iset) instrs /\
       (imem ml.(code_start) ml.(code_pastend) instrs *
        mem_available ml.(heap_start) ml.(heap_pastend) *
        mem_available ml.(stack_start) ml.(stack_pastend))%sep initial.(getMem) /\
@@ -296,280 +168,52 @@ Section Pipeline1.
                  List.In a initial.(getXAddrs)) /\
       initial.(getPc) = ml.(code_start) /\
       initial.(getNextPc) = word.add initial.(getPc) (word.of_Z 4) /\
-      regs_initialized initial.(getRegs) /\
+      FlatToRiscvCommon.regs_initialized initial.(getRegs) /\
       initial.(getLog) = nil /\
       valid_machine initial.
 
-  Lemma establish_ll_inv: forall (initial: MetricRiscvMachine),
-      initial_conditions initial ->
-      ll_inv initial.
-  Proof.
-    unfold initial_conditions.
-    intros. simp.
-    unfold ll_inv, runsToGood_Invariant.
-    destruct_RiscvMachine initial.
-    match goal with
-    | H: context[ProgramSatisfiesSpec] |- _ => rename H into sat
-    end.
-    pose proof sat.
-    destruct sat.
-    eassert ((imem ml.(code_start) ml.(code_pastend) instrs * _)%sep initial_mem) as SplitImem. {
-      ecancel_assumption.
-    }
-    destruct SplitImem as [i_mem [non_imem [SplitImem [Imem NonImem] ] ] ].
-    destruct NonImem as [heap_mem [stack_mem [SplitNonImem [HeapMem StackMem] ] ] ].
-    unfold imem in *.
-    unfold compile_prog in *.
-    remember instrs as instrs0.
-    simp.
-    rewrite instrencode_app, instrencode_cons in *.
-    unfold ptsto_bytes in *.
-    assert (map.ok mem) by exact mem_ok.
-    assert (word.ok Semantics.word) by exact word_ok.
-    array_app_cons_sep.
-    (* first, run init_sp_code: *)
-    pose proof FlatToRiscvLiterals.compile_lit_correct_full_raw as P.
-    cbv zeta in P. (* needed for COQBUG https://github.com/coq/coq/issues/11253 *)
-    specialize P with (x := RegisterNames.sp) (v := init_sp).
-    unfold runsTo in P. eapply P; clear P; simpl.
-    { assumption. }
-    2: {
-      unfold program.
-      replace (array ptsto_instr (word.of_Z 4) initial_pc (FlatToRiscvDef.compile_lit RegisterNames.sp init_sp))
-        with (array ptsto (word.of_Z 1) (code_start ml)
-                    (instrencode (FlatToRiscvDef.compile_lit RegisterNames.sp init_sp))). 2: {
-        case TODO_sam. (* need general ptsto_instr/program to ptsto instrencode conversion *)
-      }
-      wcancel_assumption.
-      cancel_seps_at_indices 2%nat 0%nat. {
-        reflexivity.
-      }
-      cbn [seps]. reflexivity.
-    }
-    {
-      assert (subset
-                (fun a => word.unsigned (code_start ml) <= word.unsigned a < word.unsigned (code_pastend ml))
-                (of_list initial_xaddrs)) as S1. {
-        unfold subset, elem_of. intros a B.
-        match goal with
-        | H: forall _, _ <= _ < _ -> _ |- _ => eapply H
-        end.
-        exact B.
-      }
-      assert (subset_trans: forall (T: Type) (s1 s2 s3: T -> Prop),
-                 subset s1 s2 -> subset s2 s3 -> subset s1 s3). {
-        clear. unfold subset, elem_of in *. intros. eauto.
-      }
-      eapply subset_trans; clear subset_trans.
-      2: exact S1.
-      clear S1.
-      eapply shrink_footpr_subset. {
-        eapply footpr_imem_range with (instrs := instrs).
-      }
-      unfold imem. subst instrs.
-      rewrite ?instrencode_app, ?instrencode_cons.
-      unfold ptsto_bytes.
-      array_app_cons_sep.
-      subst.
-      simpl.
-      wcancel.
-      unfold program.
-      replace (array ptsto_instr (word.of_Z 4) ml.(code_start) (FlatToRiscvDef.compile_lit RegisterNames.sp init_sp))
-        with (array ptsto (word.of_Z 1) (code_start ml)
-                    (instrencode (FlatToRiscvDef.compile_lit RegisterNames.sp init_sp))). 2: {
-        case TODO_sam. (* need general ptsto_instr/program to ptsto instrencode conversion *)
-      }
-      cbn [seps].
-      wcancel.
-      case TODO_sam. (* don't make such a mess *)
-    }
-    { cbv. auto. }
-    { assumption. }
-    specialize init_code_correct with (mc0 := (bedrock2.MetricLogging.mkMetricLog 0 0 0 0)).
-    assert (exists f_entry_rel_pos, map.get positions "init"%string = Some f_entry_rel_pos) as GetPos. {
-      unfold compile, composePhases, renamePhase, flattenPhase, riscvPhase in *. simp.
-      unfold flatten_functions, rename_functions, FlatToRiscvDef.function_positions in *.
-      apply get_build_fun_pos_env.
-      eapply (map.map_all_values_not_None_fw _ _ _ _ _ E3).
-      unshelve eapply (map.map_all_values_not_None_fw _ _ _ _ _ E2).
-      1, 2: simpl; typeclasses eauto.
-      simpl in *. (* PARAMRECORDS *)
-      congruence.
-    }
-    destruct GetPos as [f_entry_rel_pos GetPos].
-    subst.
-    (* then, run init_code (using compiler simulation and correctness of init_code) *)
-    eapply runsTo_weaken.
-    - pose proof compiler_correct as P. unfold runsTo in P. (* TODO instantiate ml to smaller ml *)
-      unfold ll_good.
-      eapply P; clear P.
-      6: {
-        unfold hl_inv in init_code_correct.
-        simpl.
-        move init_code_correct at bottom.
-        subst.
-        refine (init_code_correct _ _).
-        replace (datamem_start spec) with (heap_start ml) by congruence.
-        replace (datamem_pastend spec) with (heap_pastend ml) by congruence.
-        exact HeapMem.
-      }
-      all: try eassumption.
-      unfold machine_ok.
-      unfold_RiscvMachine_get_set.
-      repeat match goal with
-             | |- exists _, _  => eexists
-             | |- _ /\ _ => split
-             | |- _ => progress cbv beta iota
-             | |- _ => eassumption
-             | |- _ => reflexivity
-             end.
-      + case TODO_sam. (* verify Jal *)
-      + case TODO_sam.
-      + case TODO_sam.
-      + destruct mlOk. solve_divisibleBy4.
-      + solve_word_eq word_ok.
-      + eapply @regs_initialized_put; try typeclasses eauto. (* PARAMRECORDS? *)
-        eassumption.
-      + rewrite map.get_put_same. unfold init_sp. rewrite word.of_Z_unsigned. reflexivity.
-      + case TODO_sam. (* valid_machine preserved *)
-    - cbv beta. unfold ll_good. intros. simp.
-      repeat match goal with
-             | |- exists _, _  => eexists
-             | |- _ /\ _ => split
-             | |- _ => progress cbv beta iota
-             | |- _ => eassumption
-             | |- _ => reflexivity
-             end.
-      + case TODO_sam.
-      + (* TODO fix memory layout (one which focuses on init instructions) *)
-        case TODO_sam.
-    Unshelve. all: intros; try exact True; try exact 0; try exact mem_ok; try apply @nil.
-  Qed.
-
-  Lemma machine_ok_frame_instrs_app_l: forall p_code f_entry_rel_pos p_stack_start p_stack_pastend i1 i2
-                                              p_call pc mH Rdata Rexec mach,
-      machine_ok p_code f_entry_rel_pos p_stack_start p_stack_pastend (i1 ++ i2) p_call pc mH Rdata Rexec mach ->
-      machine_ok p_code f_entry_rel_pos p_stack_start p_stack_pastend i2 p_call pc mH Rdata
-                 (Rexec * ptsto_bytes (word.add p_code (word.of_Z (4 * Z.of_nat (List.length i1))))
-                                      (instrencode i2))%sep
-                 mach.
-  Proof.
-    unfold machine_ok.
-    intros. simp.
-    ssplit; eauto.
-    all: case TODO_sam.
-  Qed.
-
-  Lemma ll_inv_is_invariant: forall (st: MetricRiscvMachine),
-      ll_inv st -> GoFlatToRiscv.mcomp_sat (run1 iset) st ll_inv.
-  Proof.
-    intros st. unfold ll_inv.
-    eapply runsToGood_is_Invariant with (jump := - 4) (pc_start := loop_pos)
-                                        (pc_end := word.add loop_pos (word.of_Z 4)).
-    - intro D.
-      apply (f_equal word.unsigned) in D.
-      rewrite word.unsigned_add in D.
-      unshelve erewrite @word.unsigned_of_Z in D. 1: exact word_ok. (* PARAMRECORDS? *)
-      unfold word.wrap in D.
-      rewrite (Z.mod_small 4) in D; cycle 1. {
-        simpl. pose proof four_fits. blia.
-      }
-      rewrite Z.mod_eq in D by apply pow2width_nonzero.
-      let ww := lazymatch type of D with context [(2 ^ ?ww)] => ww end in set (w := ww) in *.
-      progress replace w with (w - 2 + 2) in D at 3 by blia.
-      rewrite Z.pow_add_r in D by (subst w; destruct width_cases as [E | E]; simpl in *; blia).
-      change (2 ^ 2) with 4 in D.
-      match type of D with
-      | ?x = ?x + 4 - ?A * 4 * ?B => assert (A * B = 1) as C by blia
-      end.
-      apply Z.eq_mul_1 in C.
-      destruct C as [C | C];
-        subst w; destruct width_cases as [E | E]; simpl in *; rewrite E in C; cbv in C; discriminate C.
-    - intros.
-      unfold ll_good, machine_ok in *.
-      simp.
-      etransitivity. 1: eassumption.
-      destruct done; solve_word_eq word_ok.
-    - (* Show that ll_ready (almost) ignores pc, nextPc, and metrics *)
-      intros.
-      unfold ll_good, machine_ok in *.
-      simp.
-      destr_RiscvMachine state.
-      repeat match goal with
-             | |- exists _, _  => eexists
-             | |- _ /\ _ => split
-             | |- _ => progress cbv beta iota
-             | |- _ => eassumption
-             | |- _ => reflexivity
-             end.
-      + destruct mlOk. subst. simpl in *. subst loop_pos. solve_divisibleBy4.
-      + solve_word_eq word_ok.
-      + subst. case TODO_sam. (* show that backjump preserves valid_machine *)
-    - unfold ll_good, machine_ok.
-      intros. simp. assumption.
-    - cbv. intuition discriminate.
-    - solve_divisibleBy4.
-    - solve_word_eq word_ok.
-    - unfold ll_good, machine_ok.
-      intros. simp. split.
-      + eexists. case TODO_sam.
-      + case TODO_sam. (* TODO the jump back Jal has to be in xframe *)
-    - (* use compiler correctness for loop body *)
-      intros.
-      unfold ll_good in *. simp.
-      match goal with
-      | H: ProgramSatisfiesSpec _ _ _ _ |- _ => pose proof H as sat; destruct H
-      end.
-      unfold hl_inv in loop_body_correct.
-      specialize loop_body_correct with (l := map.empty) (mc := bedrock2.MetricLogging.mkMetricLog 0 0 0 0).
-      lazymatch goal with
-      | H: context[@word.add ?w ?wo ?x (word.of_Z 0)] |- _ =>
-        replace (@word.add w wo x (word.of_Z 0)) with x in H
-      end.
-      2: {
-        (* PARAMRECORDS *)
-        symmetry. unshelve eapply SimplWordExpr.add_0_r.
-      }
-      subst.
-      match goal with
-      | H: _ |- _ => pose proof H; apply compile_prog_to_compile in H;
-                     destruct H as [ before [ finstrs [ ? ? ] ] ]
-      end.
-      subst.
-      eapply runsTo_weaken.
-      + pose proof compiler_correct as P. unfold runsTo in P.
-        eapply P; clear P. 6: {
-          eapply loop_body_correct; eauto.
-        }
-        all: try eassumption.
-        eapply machine_ok_frame_instrs_app_l. eassumption.
-      + cbv beta.
-        intros. simp. do 3 eexists.
-        ssplit; try eassumption.
-        eexists.
-        split; [eassumption|].
-        split; [eassumption|].
-        case TODO_sam. (* similar to machine_ok_frame_instrs_app_l *)
-    Unshelve. all: case TODO_sam.
-  Qed.
-
-  Lemma ll_inv_implies_prefix_of_good: forall st,
-      ll_inv st -> exists suff, spec.(goodTrace) (suff ++ st.(getLog)).
-  Proof.
-    unfold ll_inv, runsToGood_Invariant. intros. simp.
-    eapply extend_runsTo_to_good_trace. 2: case TODO_sam. 2: eassumption.
-    simpl. unfold ll_good, compile_inv, related, hl_inv,
-           compose_relation, FlattenExprSimulation.related,
-           RegRename.related, FlatToRiscvSimulation.related, FlatToRiscvFunctions.goodMachine.
-    intros. simp. eassumption.
-  Qed.
-
   Lemma compiler_invariant_proofs:
-    (forall initial, initial_conditions initial -> ll_inv initial) /\
-    (forall st, ll_inv st -> GoFlatToRiscv.mcomp_sat (run1 iset) st ll_inv) /\
-    (forall st, ll_inv st -> exists suff, spec.(goodTrace) (suff ++ st.(getLog))).
+    (forall initial, initial_conditions initial -> ll_inv ml spec initial) /\
+    (forall st, ll_inv ml spec st -> GoFlatToRiscv.mcomp_sat (run1 iset) st (ll_inv ml spec)) /\
+    (forall st, ll_inv ml spec st -> exists suff, spec.(goodTrace) (suff ++ st.(getLog))).
   Proof.
-    eauto 7 using establish_ll_inv, ll_inv_is_invariant, ll_inv_implies_prefix_of_good.
+    assert (map.ok Pipeline.mem) as Okk by exact FlatToRiscvCommon.mem_ok. (* PARAMRECORDS *)
+    ssplit; intros.
+    - eapply establish_ll_inv. 1: assumption.
+      unfold initial_conditions, ToplevelLoop.initial_conditions in *.
+      simp.
+      eassert ((ptsto_bytes (code_start ml) (instrencode instrs) * _)%sep initial.(getMem)) as SplitImem. {
+        unfold imem in *.
+        (* PARAMRECORDS *)
+        simpl in *.
+        assert (word.ok Semantics.word) by exact word_ok.
+        ecancel_assumption.
+      }
+      destruct SplitImem as [i_mem [non_imem [SplitImem [Imem NonImem] ] ] ].
+      do 4 eexists.
+      ssplit; try eassumption.
+      + unfold subset, footpr, footprint_underapprox, of_list, elem_of, program.
+        intros a M.
+        match goal with
+        | H: _ |- _ => eapply H
+        end.
+        specialize (M i_mem).
+        destruct mlOk.
+        destruct M as [v M].
+        * apply ptsto_bytes_to_program; assumption.
+        * unfold ptsto_bytes in Imem.
+          eapply ptsto_bytes_range; try eassumption.
+      + assert (word.ok Semantics.word) as Ok by exact word_ok.
+        simpl in *.
+        unfold imem in *.
+        wcancel_assumption.
+        unfold ptsto_bytes.
+        cancel_seps_at_indices 0%nat 0%nat. 2: reflexivity.
+        eapply iff1ToEq.
+        destruct mlOk.
+        eapply ptsto_bytes_to_program; try eassumption.
+    - eapply @ll_inv_is_invariant; eassumption.
+    - eapply ll_inv_implies_prefix_of_good. eassumption.
   Qed.
 
 End Pipeline1.
