compiler/src/compiler/ToplevelLoop.v
@@ -1,0 +1,368 @@
+Require Export Coq.Lists.List.
+Require Import Coq.ZArith.ZArith.
+Export ListNotations.
+Require Export coqutil.Decidable.
+Require Import coqutil.Tactics.rewr.
+Require        compiler.ExprImp.
+Require Export compiler.FlattenExprDef.
+Require Export compiler.FlattenExpr.
+Require        compiler.FlatImp.
+Require Export riscv.Spec.Decode.
+Require Export riscv.Spec.Machine.
+Require Export riscv.Platform.Run.
+Require Export riscv.Platform.Minimal.
+Require Export riscv.Platform.MetricLogging.
+Require Export riscv.Utility.Monads.
+Require Import riscv.Utility.runsToNonDet.
+Require Export riscv.Platform.MetricRiscvMachine.
+Require Import coqutil.Z.Lia.
+Require Import compiler.NameGen.
+Require Import compiler.StringNameGen.
+Require Export compiler.util.Common.
+Require Export coqutil.Decidable.
+Require Export riscv.Utility.Encode.
+Require Export riscv.Spec.Primitives.
+Require Export riscv.Spec.MetricPrimitives.
+Require Import compiler.GoFlatToRiscv.
+Require Import riscv.Utility.MkMachineWidth.
+Require Export riscv.Proofs.DecodeEncode.
+Require Export riscv.Proofs.EncodeBound.
+Require Export compiler.EmitsValid.
+Require coqutil.Map.SortedList.
+Require Import riscv.Utility.Utility.
+Require Export riscv.Platform.Memory.
+Require Export riscv.Utility.InstructionCoercions.
+Require Import compiler.SeparationLogic.
+Require Import compiler.Simp.
+Require Import compiler.FlattenExprSimulation.
+Require Import compiler.RegRename.
+Require Import compiler.FlatToRiscvSimulation.
+Require Import compiler.Simulation.
+Require Import compiler.RiscvEventLoop.
+Require Import bedrock2.MetricLogging.
+Require Import compiler.FlatToRiscvCommon.
+Require Import compiler.FlatToRiscvFunctions.
+Require Import compiler.DivisibleBy4.
+Require Import compiler.SimplWordExpr.
+Require Import compiler.ForeverSafe.
+Require Export compiler.MemoryLayout.
+Require Import FunctionalExtensionality.
+Require Import coqutil.Tactics.autoforward.
+Require Import compiler.FitsStack.
+Require Import compiler.PipelineWithRename.
+Require Import compiler.ExprImpEventLoopSpec.
+
+Existing Instance riscv.Spec.Machine.DefaultRiscvState.
+
+Open Scope Z_scope.
+
+Local Open Scope ilist_scope.
+
+Local Notation "' x <- a ; f" :=
+  (match (a: option _) with
+   | x => f
+   | _ => None
+   end)
+  (right associativity, at level 70, x pattern).
+
+Local Axiom TODO_sam: False.
+
+Section Pipeline1.
+
+  Context {p: Pipeline.parameters}.
+  Context {h: Pipeline.assumptions}.
+
+  Context (ml: MemoryLayout)
+          (mlOk: MemoryLayoutOk ml).
+
+  Let init_sp := word.unsigned ml.(stack_pastend).
+
+  Local Notation source_env := (@Pipeline.string_keyed_map p (list string * list string * Syntax.cmd)).
+
+  (* All riscv machine code, layed out from low to high addresses:
+     - init_sp_insts: initializes stack pointer
+     - init_insts: calls init function
+     - loop_insts: calls loop function
+     - backjump_insts: jumps back to calling loop function
+     - fun_insts: code of compiled functions *)
+  Definition compile_prog(prog: source_env): option (list Instruction * funname_env Z) :=
+    'Some (fun_insts, positions) <- @compile p ml prog;
+    let init_sp_insts := FlatToRiscvDef.compile_lit RegisterNames.sp init_sp in
+    'Some init_pos <- map.get positions "init"%string;
+    'Some loop_pos <- map.get positions "loop"%string;
+    let init_insts := [[Jal RegisterNames.ra (3 * 4 + init_pos)]] in
+    let loop_insts := [[Jal RegisterNames.ra (2 * 4 + loop_pos)]] in
+    let backjump_insts := [[Jal Register0 (-4*Z.of_nat (List.length loop_insts))]] in
+    Some (init_sp_insts ++ init_insts ++ loop_insts ++ backjump_insts ++ fun_insts, positions).
+
+  Context (spec: @ProgramSpec (FlattenExpr.mk_Semantics_params _)).
+
+  Let loop_pos := word.add ml.(code_start)
+         (word.of_Z (4 * (Z.of_nat (List.length (FlatToRiscvDef.compile_lit RegisterNames.sp init_sp))) + 4)).
+
+  Axiom Rdata: mem -> Prop. (* maybe (emp True) will be fine *)
+  Axiom Rexec: mem -> Prop. (* maybe (emp True) will be fine *)
+
+  Definition ll_good(done: bool)(mach: MetricRiscvMachine): Prop :=
+    exists (prog: source_env) (instrs: list Instruction) (positions: funname_env Z) (loop_fun_pos: Z),
+      compile_prog prog = Some (instrs, positions) /\
+      ProgramSatisfiesSpec "init"%string "loop"%string prog spec /\
+      map.get positions "loop"%string = Some loop_fun_pos /\
+      exists mH,
+        isReady spec mach.(getLog) mH /\ goodTrace spec mach.(getLog) /\
+        machine_ok ml.(code_start) loop_fun_pos ml.(stack_start) ml.(stack_pastend) instrs
+                   loop_pos (word.add loop_pos (word.of_Z (if done then 4 else 0))) mH Rdata Rexec mach.
+
+  Definition ll_inv: MetricRiscvMachine -> Prop := runsToGood_Invariant ll_good.
+
+  Add Ring wring : (word.ring_theory (word := Utility.word))
+      (preprocess [autorewrite with rew_word_morphism],
+       morphism (word.ring_morph (word := Utility.word)),
+       constants [word_cst]).
+
+  Lemma compile_prog_to_compile: forall prog instrs positions,
+      compile_prog prog = Some (instrs, positions) ->
+      exists before main,
+        compile ml prog = Some (main, positions) /\
+        instrs = before ++ main.
+  Proof.
+    intros. unfold compile_prog in *. simp. do 2 eexists.
+    split; [reflexivity|].
+    match goal with
+    | |- ?A ++ ?i1 :: ?i2 :: ?i3 :: ?B = ?R => change (A ++ [i1; i2; i3] ++ B = R)
+    end.
+    rewrite app_assoc.
+    reflexivity.
+  Qed.
+
+  Definition initial_conditions(initial: MetricRiscvMachine): Prop :=
+    exists (srcprog: source_env) (instrs: list Instruction) (positions: funname_env Z) (R: mem -> Prop),
+      ProgramSatisfiesSpec "init"%string "loop"%string srcprog spec /\
+      spec.(datamem_start) = ml.(heap_start) /\
+      spec.(datamem_pastend) = ml.(heap_pastend) /\
+      compile_prog srcprog = Some (instrs, positions) /\
+      subset (footpr (program ml.(code_start) instrs)) (of_list initial.(getXAddrs)) /\
+      (program ml.(code_start) instrs * R *
+       mem_available ml.(heap_start) ml.(heap_pastend) *
+       mem_available ml.(stack_start) ml.(stack_pastend))%sep initial.(getMem) /\
+      initial.(getPc) = ml.(code_start) /\
+      initial.(getNextPc) = word.add initial.(getPc) (word.of_Z 4) /\
+      regs_initialized initial.(getRegs) /\
+      initial.(getLog) = nil /\
+      valid_machine initial.
+
+  Lemma establish_ll_inv: forall (initial: MetricRiscvMachine),
+      initial_conditions initial ->
+      ll_inv initial.
+  Proof.
+    unfold initial_conditions.
+    intros. simp.
+    unfold ll_inv, runsToGood_Invariant.
+    destruct_RiscvMachine initial.
+    match goal with
+    | H: context[ProgramSatisfiesSpec] |- _ => rename H into sat
+    end.
+    pose proof sat.
+    destruct sat.
+    match goal with
+    | H: compile_prog srcprog = Some _ |- _ => pose proof H as CP; unfold compile_prog in H
+    end.
+    remember instrs as instrs0.
+    simp.
+    assert (map.ok mem) by exact mem_ok.
+    assert (word.ok Semantics.word) by exact word_ok.
+    eassert ((mem_available ml.(heap_start) ml.(heap_pastend) * _)%sep initial_mem) as SplitImem. {
+      ecancel_assumption.
+    }
+    destruct SplitImem as [heap_mem [other_imem [SplitHmem [HMem OtherMem] ] ] ].
+    (* first, run init_sp_code: *)
+    pose proof FlatToRiscvLiterals.compile_lit_correct_full_raw as P.
+    cbv zeta in P. (* needed for COQBUG https://github.com/coq/coq/issues/11253 *)
+    specialize P with (x := RegisterNames.sp) (v := init_sp) (Rexec := emp True).
+    unfold runsTo in P. eapply P; clear P; simpl.
+    { assumption. }
+    2: { wcancel_assumption. }
+    {
+      eapply shrink_footpr_subset. 1: eassumption.
+      wwcancel.
+    }
+    { cbv. auto. }
+    { assumption. }
+    specialize init_code_correct with (mc0 := (bedrock2.MetricLogging.mkMetricLog 0 0 0 0)).
+    assert (exists f_entry_rel_pos, map.get positions "init"%string = Some f_entry_rel_pos) as GetPos. {
+      unfold compile, composePhases, renamePhase, flattenPhase, riscvPhase in *. simp.
+      unfold flatten_functions, rename_functions, FlatToRiscvDef.function_positions in *.
+      apply get_build_fun_pos_env.
+      eapply (map.map_all_values_not_None_fw _ _ _ _ _ E3).
+      unshelve eapply (map.map_all_values_not_None_fw _ _ _ _ _ E2).
+      1, 2: simpl; typeclasses eauto.
+      simpl in *. (* PARAMRECORDS *)
+      congruence.
+    }
+    destruct GetPos as [f_entry_rel_pos GetPos].
+    subst.
+    (* then, run init_code (using compiler simulation and correctness of init_code) *)
+    eapply runsTo_weaken.
+    - pose proof compiler_correct as P. unfold runsTo in P. (* TODO instantiate ml to smaller ml *)
+      unfold ll_good.
+      eapply P; clear P.
+      6: {
+        unfold hl_inv in init_code_correct.
+        simpl.
+        move init_code_correct at bottom.
+        subst.
+        refine (init_code_correct _ _).
+        replace (datamem_start spec) with (heap_start ml) by congruence.
+        replace (datamem_pastend spec) with (heap_pastend ml) by congruence.
+        exact HMem.
+      }
+      all: try eassumption.
+      unfold machine_ok.
+      unfold_RiscvMachine_get_set.
+      repeat match goal with
+             | |- exists _, _  => eexists
+             | |- _ /\ _ => split
+             | |- _ => progress cbv beta iota
+             | |- _ => eassumption
+             | |- _ => reflexivity
+             end.
+      + case TODO_sam. (* verify Jal *)
+      + case TODO_sam.
+      + case TODO_sam.
+      + destruct mlOk. solve_divisibleBy4.
+      + solve_word_eq word_ok.
+      + eapply @regs_initialized_put; try typeclasses eauto. (* PARAMRECORDS? *)
+        eassumption.
+      + rewrite map.get_put_same. unfold init_sp. rewrite word.of_Z_unsigned. reflexivity.
+      + case TODO_sam. (* valid_machine preserved *)
+    - cbv beta. unfold ll_good. intros. simp.
+      repeat match goal with
+             | |- exists _, _  => eexists
+             | |- _ /\ _ => split
+             | |- _ => progress cbv beta iota
+             | |- _ => eassumption
+             | |- _ => reflexivity
+             end.
+      + (* TODO fix memory layout (one which focuses on init instructions) *)
+        case TODO_sam.
+    Unshelve. all: intros; try exact True; try exact 0; try exact mem_ok; try apply @nil.
+  Qed.
+
+  Lemma machine_ok_frame_instrs_app_l: forall p_code f_entry_rel_pos p_stack_start p_stack_pastend i1 i2
+                                              p_call pc mH Rdata Rexec mach,
+      machine_ok p_code f_entry_rel_pos p_stack_start p_stack_pastend (i1 ++ i2) p_call pc mH Rdata Rexec mach ->
+      machine_ok p_code f_entry_rel_pos p_stack_start p_stack_pastend i2 p_call pc mH Rdata
+                 (Rexec * program (word.add p_code (word.of_Z (4 * Z.of_nat (List.length i1))))i2)%sep
+                 mach.
+  Proof.
+    unfold machine_ok.
+    intros. simp.
+    ssplit; eauto.
+    all: case TODO_sam.
+  Qed.
+
+  Lemma ll_inv_is_invariant: forall (st: MetricRiscvMachine),
+      ll_inv st -> GoFlatToRiscv.mcomp_sat (run1 iset) st ll_inv.
+  Proof.
+    intros st. unfold ll_inv.
+    eapply runsToGood_is_Invariant with (jump := - 4) (pc_start := loop_pos)
+                                        (pc_end := word.add loop_pos (word.of_Z 4)).
+    - intro D.
+      apply (f_equal word.unsigned) in D.
+      rewrite word.unsigned_add in D.
+      unshelve erewrite @word.unsigned_of_Z in D. 1: exact word_ok. (* PARAMRECORDS? *)
+      unfold word.wrap in D.
+      rewrite (Z.mod_small 4) in D; cycle 1. {
+        simpl. pose proof four_fits. blia.
+      }
+      rewrite Z.mod_eq in D by apply pow2width_nonzero.
+      let ww := lazymatch type of D with context [(2 ^ ?ww)] => ww end in set (w := ww) in *.
+      progress replace w with (w - 2 + 2) in D at 3 by blia.
+      rewrite Z.pow_add_r in D by (subst w; destruct width_cases as [E | E]; simpl in *; blia).
+      change (2 ^ 2) with 4 in D.
+      match type of D with
+      | ?x = ?x + 4 - ?A * 4 * ?B => assert (A * B = 1) as C by blia
+      end.
+      apply Z.eq_mul_1 in C.
+      destruct C as [C | C];
+        subst w; destruct width_cases as [E | E]; simpl in *; rewrite E in C; cbv in C; discriminate C.
+    - intros.
+      unfold ll_good, machine_ok in *.
+      simp.
+      etransitivity. 1: eassumption.
+      destruct done; solve_word_eq word_ok.
+    - (* Show that ll_ready (almost) ignores pc, nextPc, and metrics *)
+      intros.
+      unfold ll_good, machine_ok in *.
+      simp.
+      destr_RiscvMachine state.
+      repeat match goal with
+             | |- exists _, _  => eexists
+             | |- _ /\ _ => split
+             | |- _ => progress cbv beta iota
+             | |- _ => eassumption
+             | |- _ => reflexivity
+             end.
+      + destruct mlOk. subst. simpl in *. subst loop_pos. solve_divisibleBy4.
+      + solve_word_eq word_ok.
+      + subst. case TODO_sam. (* show that backjump preserves valid_machine *)
+    - unfold ll_good, machine_ok.
+      intros. simp. assumption.
+    - cbv. intuition discriminate.
+    - solve_divisibleBy4.
+    - solve_word_eq word_ok.
+    - unfold ll_good, machine_ok.
+      intros. simp. split.
+      + eexists. case TODO_sam.
+      + case TODO_sam. (* TODO the jump back Jal has to be in xframe *)
+    - (* use compiler correctness for loop body *)
+      intros.
+      unfold ll_good in *. simp.
+      match goal with
+      | H: ProgramSatisfiesSpec _ _ _ _ |- _ => pose proof H as sat; destruct H
+      end.
+      unfold hl_inv in loop_body_correct.
+      specialize loop_body_correct with (l := map.empty) (mc := bedrock2.MetricLogging.mkMetricLog 0 0 0 0).
+      lazymatch goal with
+      | H: context[@word.add ?w ?wo ?x (word.of_Z 0)] |- _ =>
+        replace (@word.add w wo x (word.of_Z 0)) with x in H
+      end.
+      2: {
+        (* PARAMRECORDS *)
+        symmetry. unshelve eapply SimplWordExpr.add_0_r.
+      }
+      subst.
+      match goal with
+      | H: _ |- _ => pose proof H; apply compile_prog_to_compile in H;
+                     destruct H as [ before [ finstrs [ ? ? ] ] ]
+      end.
+      subst.
+      eapply runsTo_weaken.
+      + pose proof compiler_correct as P. unfold runsTo in P.
+        eapply P; clear P. 6: {
+          eapply loop_body_correct; eauto.
+        }
+        all: try eassumption.
+        eapply machine_ok_frame_instrs_app_l. eassumption.
+      + cbv beta.
+        intros. simp. do 3 eexists.
+        ssplit; try eassumption.
+        eexists.
+        split; [eassumption|].
+        split; [eassumption|].
+        case TODO_sam. (* similar to machine_ok_frame_instrs_app_l *)
+    Unshelve. all: case TODO_sam.
+  Qed.
+
+  Lemma ll_inv_implies_prefix_of_good: forall st,
+      ll_inv st -> exists suff, spec.(goodTrace) (suff ++ st.(getLog)).
+  Proof.
+    unfold ll_inv, runsToGood_Invariant. intros. simp.
+    eapply extend_runsTo_to_good_trace. 2: case TODO_sam. 2: eassumption.
+    simpl. unfold ll_good, compile_inv, related, hl_inv,
+           compose_relation, FlattenExprSimulation.related,
+           RegRename.related, FlatToRiscvSimulation.related, FlatToRiscvFunctions.goodMachine.
+    intros. simp. eassumption.
+  Qed.
+
+End Pipeline1.
